theories/PCFm.v
@@ -25,7 +25,7 @@ Arguments Absₘ {μ Γ α}.
 Set Elimination Schemes.
 
 Notation "s  '$ₘ'  t" := (Appₘ s t) (at level 40, left associativity).
-Notation "'λₘ:'  α ','  s" := (Absₘ α s) (at level 35, s at level 200).
+Notation "'λₘ:'  α ','  s" := (Absₘ α s) (at level 60, s at level 60, right associativity).
 
 Definition termₘ_rect (μ : nat) (P : ∀ Γ α, termₘ μ Γ α → Type)
   (case_kₘ : ∀ Γ n, P Γ ι (kₘ n))
@@ -74,6 +74,13 @@ Definition termₘ_rec (μ : nat) (P : ∀ Γ α, termₘ μ Γ α → Set) := t
 Equations Derive Signature for termₘ.
 Equations Derive NoConfusion for termₘ.
 
+Instance arbitrary_termₘ {μ Γ α} : Arbitrary (termₘ μ Γ α).
+Proof.
+  revert Γ; induction α as [| α' IH_α' β' IH_β']; intros Γ.
+  - apply (kₘ (Zm_of_Z 0%Z)).
+  - apply Absₘ. apply IH_β'.
+Defined.
+
 Instance dec_eq_termₘ {μ Γ α} : EqDec (termₘ μ Γ α) eq.
 Proof.
   rewrite dec_eq_def.
@@ -82,7 +89,7 @@ Proof.
     destruct (n_1 == n_2) as [H_n | H_n]; constructor; congruence.
   - ltac1:(dependent elimination s_2 as [@Pₘ Γ_2 | @Sₘ Γ_2 | @Varₘ Γ_2 α_2 mi_2 | @Appₘ Γ_2 α_2 β_2 s'_2 t'_2 | @Absₘ Γ_2 α_2 β_2 s'_2]); constructor; congruence.
   - ltac1:(dependent elimination s_2 as [@Pₘ Γ_2 | @Sₘ Γ_2 | @Varₘ Γ_2 α_2 mi_2 | @Appₘ Γ_2 α_2 β_2 s'_2 t'_2 | @Absₘ Γ_2 α_2 β_2 s'_2]); constructor; congruence.
-  - ltac1:(dependent elimination s_2 as [@kₘ Γ_ n_2 | @switchₘ Γ_2 s'_2 f_2 | @Varₘ Γ_2 α_2 mi_2 | @Appₘ Γ_2 α_2 β_2 s'_2 t'_2]); try (right; congruence).
+  - ltac1:(dependent elimination s_2 as [@kₘ Γ_2 n_2 | @switchₘ Γ_2 s'_2 f_2 | @Varₘ Γ_2 α_2 mi_2 | @Appₘ Γ_2 α_2 β_2 s'_2 t'_2]); try (right; congruence).
     specialize (IH_s' s'_2). ltac1:(pose proof (IH'_f := λ n, IH_f n (f_2 n))); clear IH_f.
     assert (H_f_default : {stabilizing_fun_default f_1 = stabilizing_fun_default f_2} + {stabilizing_fun_default f_1 ≠ stabilizing_fun_default f_2}). {
       remember (stabilizing_fun_default f_1) as f_default_1 eqn:H_f_default_1; remember (stabilizing_fun_default f_2) as f_default_2 eqn:H_f_default_2. destruct f_default_1 as [t'_1 |], f_default_2 as [t'_2 |]; try (right; congruence).
@@ -92,9 +99,9 @@ Proof.
     ltac1:(pose proof (H_f := dec_eq_stabilizing_fun_minimal f_1 f_2 IH'_f H_f_default)).
     destruct IH_s' as [IH_s' | IH_s'] > [destruct H_f as [H_f | H_f] |]; constructor; congruence.
   - ltac1:(dependent elimination s_2 as [@fixₘ Γ_2 α_2 | @Varₘ Γ_2 α_2 mi_2 | @Appₘ Γ_2 α_2 β_2 s'_2 t'_2 | @Absₘ Γ_2 α_2 β_2 s'_2]); constructor; congruence.
-  - ltac1:(dependent elimination s_2 as [@kₘ Γ_ n_2 | @Pₘ Γ_2 | @Sₘ Γ_2 | @switchₘ Γ_2 s'_2 f_2 | @fixₘ Γ_2 α_2 | @Varₘ Γ_2 α_2 mi_2 | @Appₘ Γ_2 α_2 β_2 s'_2 t'_2 | @Absₘ Γ_2 α_2 β_2 s'_2]); try (right; congruence).
+  - ltac1:(dependent elimination s_2 as [@kₘ Γ_2 n_2 | @Pₘ Γ_2 | @Sₘ Γ_2 | @switchₘ Γ_2 s'_2 f_2 | @fixₘ Γ_2 α_2 | @Varₘ Γ_2 α_2 mi_2 | @Appₘ Γ_2 α_2 β_2 s'_2 t'_2 | @Absₘ Γ_2 α_2 β_2 s'_2]); try (right; congruence).
     destruct (mi_1 == mi_2 : {_ = _} + {_ ≠ _}) as [-> | H_mi]; constructor; congruence.
-  - ltac1:(dependent elimination s_2 as [@kₘ Γ_ n_2 | @Pₘ Γ_2 | @Sₘ Γ_2 | @switchₘ Γ_2 s'_2 f_2 | @fixₘ Γ_2 α_2 | @Varₘ Γ_2 α_2 mi_2 | @Appₘ Γ_2 α_2 β_2 s'_2 t'_2 | @Absₘ Γ_2 α_2 β_2 s'_2]); try (right; congruence).
+  - ltac1:(dependent elimination s_2 as [@kₘ Γ_2 n_2 | @Pₘ Γ_2 | @Sₘ Γ_2 | @switchₘ Γ_2 s'_2 f_2 | @fixₘ Γ_2 α_2 | @Varₘ Γ_2 α_2 mi_2 | @Appₘ Γ_2 α_2 β_2 s'_2 t'_2 | @Absₘ Γ_2 α_2 β_2 s'_2]); try (right; congruence).
     destruct (α_1 == α_2) as [-> | H_α]; try (right; congruence). specialize (IH_s' s'_2). specialize (IH_t' t'_2).
     destruct IH_s' as [IH_s' | IH_s'] > [destruct IH_t' as [IH_t' | IH_t'] |].
     + left; congruence.
@@ -111,6 +118,10 @@ Inductive termₘ_direct_subterm {μ} : ∀ {Γ_1 α_1 Γ_2 α_2}, termₘ μ Γ
   | termₘ_direct_subterm_switchₘ_f :
     ∀ {Γ} (s' : termₘ μ Γ ι) (f : Zm μ →₀ termₘ μ Γ ι) n,
     termₘ_direct_subterm (f n) (switchₘ s' f)
+  | termₘ_direct_subterm_switchₘ_f_default :
+    ∀ {Γ} (s' : termₘ μ Γ ι) (f : Zm μ →₀ termₘ μ Γ ι) (t' : termₘ μ Γ ι),
+    stabilizing_fun_default f = Some t' →
+    termₘ_direct_subterm t' (switchₘ s' f)
   | termₘ_direct_subterm_Appₘ_s' :
     ∀ {Γ α β} (s' : termₘ μ Γ (α ⇒ β)) (t' : termₘ μ Γ α),
     termₘ_direct_subterm s' (s' $ₘ t')
@@ -123,6 +134,7 @@ Inductive termₘ_direct_subterm {μ} : ∀ {Γ_1 α_1 Γ_2 α_2}, termₘ μ Γ
 
 Hint Resolve termₘ_direct_subterm_switchₘ_s' : subterm_relation.
 Hint Resolve termₘ_direct_subterm_switchₘ_f : subterm_relation.
+Hint Resolve termₘ_direct_subterm_switchₘ_f_default : subterm_relation.
 Hint Resolve termₘ_direct_subterm_Appₘ_s' : subterm_relation.
 Hint Resolve termₘ_direct_subterm_Appₘ_t' : subterm_relation.
 Hint Resolve termₘ_direct_subterm_Absₘ_s' : subterm_relation.
@@ -137,7 +149,8 @@ Hint Unfold termₘ_subterm : subterm_relation.
 Instance well_founded_termₘ_subterm {μ} : WellFounded (@termₘ_subterm μ).
 Proof.
   apply Transitive_Closure.wf_clos_trans. intros [[Γ_1 α_1] s_1]; simpl in s_1.
-  induction s_1 as [Γ_1 n_1 | Γ_1 | Γ_1 | Γ_1 s'_1 IH_s' f_1 IH_f IH_f_default | Γ_1 α_1 | Γ_1 α_1 mi_1 | Γ_1 α_1 β_1 s'_1 IH_s' t'_1 IH_t' | Γ_1 α_1 β_1 s'_1 IH_s']; apply Acc_intro; simpl; intros [[Γ_2 α_2] s_2] H; simpl in s_2 |- *; try (solve [ltac1:(dependent elimination s_2 as [@kₘ Γ_2 n_2 | @Pₘ Γ_2 | @Sₘ Γ_2 | @switchₘ Γ_2 s'_2 f_2 | @fixₘ Γ_2 α_2 | @Varₘ Γ_2 α_2 mi_2 | @Appₘ Γ_2 α_2_ β_2 s'_2 t'_2 | @Absₘ Γ_2 α_2 β_2 s'_2]); inversion H]); ltac1:(dependent elimination H); auto.
+  induction s_1 as [Γ_1 n_1 | Γ_1 | Γ_1 | Γ_1 s'_1 IH_s' f_1 IH_f IH_f_default | Γ_1 α_1 | Γ_1 α_1 mi_1 | Γ_1 α_1 β_1 s'_1 IH_s' t'_1 IH_t' | Γ_1 α_1 β_1 s'_1 IH_s']; apply Acc_intro; simpl; intros [[Γ_2 α_2] s_2] H; simpl in s_2 |- *; try (solve [ltac1:(dependent elimination s_2 as [@kₘ Γ_2 n_2 | @Pₘ Γ_2 | @Sₘ Γ_2 | @switchₘ Γ_2 s'_2 f_2 | @fixₘ Γ_2 α_2 | @Varₘ Γ_2 α_2 mi_2 | @Appₘ Γ_2 α_2_ β_2 s'_2 t'_2 | @Absₘ Γ_2 α_2 β_2 s'_2]); inversion H]); try (solve[ltac1:(dependent elimination H); auto]).
+  ltac1:(dependent elimination H as [@termₘ_direct_subterm_switchₘ_s' Γ_1 s'_1 f_1 | @termₘ_direct_subterm_switchₘ_f Γ_1 s'_1 f_1 n | @termₘ_direct_subterm_switchₘ_f_default Γ_1 s'_1 f_1 t'_1 H_t'_1]); auto. destruct (stabilizing_fun_default f_1) as [x |]; congruence.
 Defined.
 
 Check (λₘ: ι, λₘ: ι, Varₘ ι (MIS MIO)) $ₘ (Sₘ $ₘ Varₘ ι MIO) $ₘ kₘ (Zm_of_Z 0%Z).
@@ -156,20 +169,51 @@ Qed.
 
 Compute ` (bool_of_sumbool (((λₘ: ι, switchₘ (Varₘ ι MIO) (Zm_of_Z 100 ↦₀ Sₘ $ₘ (Sₘ $ₘ kₘ (Zm_of_Z 0%Z)), Zm_of_Z 11 ↦₀ kₘ (Zm_of_Z 0%Z), _ ↦₀ Sₘ $ₘ kₘ (Zm_of_Z 0%Z))) : termₘ 10 [] _) == (λₘ: ι, switchₘ (Varₘ ι MIO) (Zm_of_Z 0 ↦₀ Sₘ $ₘ (Sₘ $ₘ kₘ (Zm_of_Z 0%Z)), Zm_of_Z 1 ↦₀ kₘ (Zm_of_Z 0%Z), _ ↦₀ Sₘ $ₘ kₘ (Zm_of_Z 20%Z))))).
 
+Section rebuild_termₘ.
+  Context {μ : nat}.
+
+  Equations rebuild_termₘ {Γ α} (s : termₘ μ Γ α) : termₘ μ Γ α by wf (signature_pack s) :=
+    | kₘ n => kₘ n
+    | Pₘ => Pₘ
+    | Sₘ => Sₘ
+    | switchₘ s' f =>
+      switchₘ
+        (rebuild_termₘ s')
+        (stabilizing_fun_rebuild_erased
+          (stabilizing_fun_map_minimal
+            (λ a, rebuild_termₘ (f a))
+            (match stabilizing_fun_default f as f_default return stabilizing_fun_default f = f_default → option (termₘ μ Γ ι) with
+            | Some t' => λ H_t', Some (rebuild_termₘ t')
+            | None => λ _, None
+            end eq_refl)
+            f
+            _)
+        )
+    | fixₘ α => fixₘ α
+    | Varₘ α mi => Varₘ α mi
+    | s' $ₘ t' => (rebuild_termₘ s') $ₘ (rebuild_termₘ t')
+    | λₘ: β, s' => λₘ: β, rebuild_termₘ s'.
+  Next Obligation.
+    intros Γ s' f renaming_inst_termₘ a_1 a_2 H_f_a. simpl.
+    generalize (rebuild_termₘ_obligations_obligation_2 Γ s' f a_1) as H_1, (rebuild_termₘ_obligations_obligation_2 Γ s' f a_2) as H_2; intros H_1 H_2.
+    destruct H_f_a. f_equal; apply proof_irrelevance.
+  Defined.
+End rebuild_termₘ.
+
 Definition substitutionₘ μ Γ Δ := ∀ (α : type), mem_index α Δ → termₘ μ Γ α.
 
 Definition substitutionₘ_of_renaming {μ Γ Δ} (σ : renaming Γ Δ) : substitutionₘ μ Γ Δ :=
   λ _ mi, Varₘ _ (σ _ mi).
 
-Definition substitutionₘ_id {μ Γ} : substitutionₘ μ Γ Γ :=
-  substitutionₘ_of_renaming renaming_id.
+Definition substitutionₘ_id {μ} Γ : substitutionₘ μ Γ Γ :=
+  substitutionₘ_of_renaming (renaming_id Γ).
 
 Equations substitutionₘ_cons {μ Γ Δ} α (s : termₘ μ Γ α) (σ : substitutionₘ μ Γ Δ) : substitutionₘ μ Γ (α :: Δ) :=
   | α, mi, σ, _, MIO => mi
   | α, mi, σ, _, MIS mi' => σ _ mi'.
 
-Definition substitutionₘ_shift {μ α Γ} : substitutionₘ μ (α :: Γ) Γ :=
-  substitutionₘ_of_renaming renaming_shift.
+Definition substitutionₘ_shift {μ} α Γ : substitutionₘ μ (α :: Γ) Γ :=
+  substitutionₘ_of_renaming (renaming_shift α Γ).
 
 Section renaming_inst_termₘ.
   Context {μ : nat}.
@@ -178,11 +222,21 @@ Section renaming_inst_termₘ.
     | σ, kₘ n => kₘ n
     | σ, Pₘ => Pₘ
     | σ, Sₘ => Sₘ
-    | σ, switchₘ s' f => switchₘ (renaming_inst_termₘ σ s') (stabilizing_fun_map_minimal (λ a, renaming_inst_termₘ σ (f a)) f _)
+    | σ, switchₘ s' f =>
+      switchₘ
+        (renaming_inst_termₘ σ s')
+        (stabilizing_fun_map_minimal
+          (λ a, renaming_inst_termₘ σ (f a))
+          (match stabilizing_fun_default f as f_default return stabilizing_fun_default f = f_default → option (termₘ μ Γ ι) with
+          | Some t' => λ H_t', Some (renaming_inst_termₘ σ t')
+          | None => λ _, None
+          end eq_refl)
+          f
+          _)
     | σ, fixₘ α => fixₘ α
     | σ, Varₘ α mi => Varₘ α (σ α mi)
-    | σ, Appₘ s' t' => Appₘ (renaming_inst_termₘ σ s') (renaming_inst_termₘ σ t')
-    | σ, Absₘ β s' => Absₘ β (renaming_inst_termₘ (renaming_up σ) s').
+    | σ, s' $ₘ t' => (renaming_inst_termₘ σ s') $ₘ (renaming_inst_termₘ σ t')
+    | σ, λₘ: β, s' => λₘ: β, renaming_inst_termₘ (renaming_up β σ) s'.
   Next Obligation.
     intros Γ Δ σ s' f renaming_inst_termₘ a_1 a_2 H_f_a. simpl.
     generalize (renaming_inst_termₘ_obligations_obligation_2 Δ s' f a_1) as H_1, (renaming_inst_termₘ_obligations_obligation_2 Δ s' f a_2) as H_2; intros H_1 H_2.
@@ -191,12 +245,12 @@ Section renaming_inst_termₘ.
 End renaming_inst_termₘ.
 
 Lemma renaming_inst_termₘ_equation_4' {μ : nat} :
-  ∀ (Γ Δ : list type) (σ : renaming Γ Δ) (s' : termₘ μ Δ ι) (f : Zm μ →₀ termₘ μ Δ ι),
-  renaming_inst_termₘ σ (switchₘ s' f) =
-  switchₘ (renaming_inst_termₘ σ s') (stabilizing_fun_map (renaming_inst_termₘ σ) f).
+  ∀ Γ Δ (σ : renaming Γ Δ) (s' : termₘ μ Δ ι) (f : Zm μ →₀ termₘ μ Δ ι),
+  renaming_inst_termₘ σ (switchₘ s' f) = switchₘ (renaming_inst_termₘ σ s') (stabilizing_fun_map (renaming_inst_termₘ σ) f).
 Proof.
   intros Γ Δ σ s' f. rewrite renaming_inst_termₘ_equation_4. unfold stabilizing_fun_map. do 2 f_equal.
-  apply functional_extensionality_dep; intros; apply functional_extensionality_dep; intros; apply functional_extensionality_dep; intros; apply proof_irrelevance.
+  - destruct (stabilizing_fun_default f); reflexivity.
+  - apply functional_extensionality_dep; intros; apply functional_extensionality_dep; intros; apply functional_extensionality_dep; intros; apply proof_irrelevance.
 Qed.
 
 Hint Rewrite @renaming_inst_termₘ_equation_1 : renaming_inst_termₘ'.
@@ -208,21 +262,584 @@ Hint Rewrite @renaming_inst_termₘ_equation_6 : renaming_inst_termₘ'.
 Hint Rewrite @renaming_inst_termₘ_equation_7 : renaming_inst_termₘ'.
 Hint Rewrite @renaming_inst_termₘ_equation_8 : renaming_inst_termₘ'.
 
+Definition substitutionₘ_comp_renaming {μ Γ Δ Θ} (τ : substitutionₘ μ Δ Θ) (σ : renaming Γ Δ) : substitutionₘ μ Γ Θ :=
+  λ _ mi, renaming_inst_termₘ σ (τ _ mi).
+
+Definition substitutionₘ_up {μ Γ Δ} α (σ : substitutionₘ μ Γ Δ) : substitutionₘ μ (α :: Γ) (α :: Δ) :=
+  substitutionₘ_cons α (Varₘ α MIO) (substitutionₘ_comp_renaming σ (renaming_shift α Γ)).
+
+Section substitutionₘ_inst.
+  Context {μ : nat}.
+
+  Equations substitutionₘ_inst {Γ Δ α} (σ : substitutionₘ μ Γ Δ) (s : termₘ μ Δ α) : termₘ μ Γ α by wf (signature_pack s) :=
+    | σ, kₘ n => kₘ n
+    | σ, Pₘ => Pₘ
+    | σ, Sₘ => Sₘ
+    | σ, switchₘ s' f =>
+      switchₘ
+        (substitutionₘ_inst σ s')
+        (stabilizing_fun_map_minimal
+          (λ a, substitutionₘ_inst σ (f a))
+          (match stabilizing_fun_default f as f_default return stabilizing_fun_default f = f_default → option (termₘ μ Γ ι) with
+          | Some t' => λ H_t', Some (substitutionₘ_inst σ t')
+          | None => λ _, None
+          end eq_refl)
+          f
+          _)
+    | σ, fixₘ α => fixₘ α
+    | σ, Varₘ α mi => σ α mi
+    | σ, s' $ₘ t' => (substitutionₘ_inst σ s') $ₘ (substitutionₘ_inst σ t')
+    | σ, λₘ: β, s' => λₘ: β, substitutionₘ_inst (substitutionₘ_up β σ) s'.
+  Next Obligation.
+    intros Γ Δ σ s' f substitutionₘ_inst a_1 a_2 H_f_a. simpl.
+    generalize (substitutionₘ_inst_obligations_obligation_2 Δ s' f a_1) as H_1, (substitutionₘ_inst_obligations_obligation_2 Δ s' f a_2) as H_2; intros H_1 H_2.
+    destruct H_f_a. f_equal; apply proof_irrelevance.
+  Defined.
+End substitutionₘ_inst.
+
+Lemma substitutionₘ_inst_equation_4' {μ : nat} :
+  ∀ Γ Δ (σ : substitutionₘ μ Γ Δ) (s' : termₘ μ Δ ι) (f : Zm μ →₀ termₘ μ Δ ι),
+  substitutionₘ_inst σ (switchₘ s' f) = switchₘ (substitutionₘ_inst σ s') (stabilizing_fun_map (substitutionₘ_inst σ) f).
+Proof.
+  intros Γ Δ σ s' f. rewrite substitutionₘ_inst_equation_4. unfold stabilizing_fun_map. do 2 f_equal.
+  - destruct (stabilizing_fun_default f); reflexivity.
+  - apply functional_extensionality_dep; intros; apply functional_extensionality_dep; intros; apply functional_extensionality_dep; intros; apply proof_irrelevance.
+Qed.
+
+Hint Rewrite @substitutionₘ_inst_equation_1 : substitutionₘ_inst'.
+Hint Rewrite @substitutionₘ_inst_equation_2 : substitutionₘ_inst'.
+Hint Rewrite @substitutionₘ_inst_equation_3 : substitutionₘ_inst'.
+Hint Rewrite @substitutionₘ_inst_equation_4' : substitutionₘ_inst'.
+Hint Rewrite @substitutionₘ_inst_equation_5 : substitutionₘ_inst'.
+Hint Rewrite @substitutionₘ_inst_equation_6 : substitutionₘ_inst'.
+Hint Rewrite @substitutionₘ_inst_equation_7 : substitutionₘ_inst'.
+Hint Rewrite @substitutionₘ_inst_equation_8 : substitutionₘ_inst'.
+
+Definition substitutionₘ_comp {μ Γ Δ Θ} (τ : substitutionₘ μ Δ Θ) (σ : substitutionₘ μ Γ Δ) : substitutionₘ μ Γ Θ :=
+  λ _ mi, substitutionₘ_inst σ (τ _ mi).
+
+Lemma renaming_id_def_termₘ {μ} :
+  ∀ Γ,
+  @substitutionₘ_of_renaming μ _ _ (renaming_id Γ) = substitutionₘ_id Γ.
+Proof.
+  intros Γ. reflexivity.
+Qed.
+
+Lemma renaming_cons_def_termₘ {μ Γ Δ} :
+  ∀ α (mi : mem_index α Γ) (σ : renaming Γ Δ),
+  @substitutionₘ_of_renaming μ _ _ (renaming_cons α mi σ) = substitutionₘ_cons α (Varₘ α mi) (substitutionₘ_of_renaming σ).
+Proof.
+  intros α mi σ. apply functional_extensionality_dep; intros β; apply functional_extensionality; intros mi_1.
+  unfold substitutionₘ_of_renaming. ltac1:(dependent elimination mi_1 as [@MIO Γ' | @MIS γ Γ' mi_1']); ltac1:(simp renaming_cons substitutionₘ_cons); reflexivity.
+Qed.
+
+Lemma renaming_shift_def_termₘ {μ} :
+  ∀ α Γ,
+  @substitutionₘ_of_renaming μ _ _ (renaming_shift α Γ) = substitutionₘ_shift α Γ.
+Proof.
+  intros α Γ. reflexivity.
+Qed.
+
+Lemma renaming_comp_def_termₘ {μ Γ Δ Θ} :
+  ∀ (τ : renaming Δ Θ) (σ : renaming Γ Δ),
+  @substitutionₘ_of_renaming μ _ _ (renaming_comp τ σ) = substitutionₘ_comp_renaming (substitutionₘ_of_renaming τ) σ.
+Proof.
+  intros τ σ. reflexivity.
+Qed.
+
+Lemma renaming_up_def_termₘ {μ Γ Δ} :
+  ∀ α (σ : renaming Γ Δ),
+  @substitutionₘ_of_renaming μ _ _ (renaming_up α σ) = substitutionₘ_up α (substitutionₘ_of_renaming σ).
+Proof.
+  intros α σ. unfold renaming_up, substitutionₘ_up. rewrite renaming_cons_def_termₘ, renaming_comp_def_termₘ. reflexivity.
+Qed.
+
+Lemma renaming_inst_termₘ_def {μ Γ Δ α} :
+  ∀ (σ : renaming Γ Δ) (s : termₘ μ Δ α),
+  renaming_inst_termₘ σ s = substitutionₘ_inst (substitutionₘ_of_renaming σ) s.
+Proof.
+  intros σ s. revert Γ σ; induction s as [Δ n | Δ | Δ | Δ s' IH_s' f IH_f IH_f_default | Δ α | Δ α mi | Δ α β s' IH_s' t' IH_t' | Δ α β s' IH_s']; intros Γ σ; ltac1:(simp renaming_inst_termₘ' substitutionₘ_inst'); try (congruence).
+  - rewrite IH_s'. f_equal. apply eq_stabilizing_fun_map.
+    + intros n. rewrite IH_f. reflexivity.
+    + destruct (stabilizing_fun_default f) as [t' |].
+      * simpl. rewrite IH_f_default. reflexivity.
+      * reflexivity.
+  - reflexivity.
+  - rewrite IH_s'. rewrite renaming_up_def_termₘ. reflexivity.
+Qed.
+
+Lemma substitutionₘ_comp_renaming_def {μ Γ Δ Θ} :
+  ∀ (τ : substitutionₘ μ Δ Θ) (σ : renaming Γ Δ),
+  substitutionₘ_comp_renaming τ σ = substitutionₘ_comp τ (substitutionₘ_of_renaming σ).
+Proof.
+  intros τ σ. unfold substitutionₘ_comp_renaming, substitutionₘ_comp. apply functional_extensionality_dep; intros α; apply functional_extensionality; intros mi.
+  rewrite renaming_inst_termₘ_def. reflexivity.
+Qed.
+
+Lemma substitutionₘ_up_def {μ Γ Δ} :
+  ∀ α (σ : substitutionₘ μ Γ Δ),
+  substitutionₘ_up α σ = substitutionₘ_cons α (Varₘ α MIO) (substitutionₘ_comp σ (substitutionₘ_shift α Γ)).
+Proof.
+  intros α σ. unfold substitutionₘ_up. rewrite substitutionₘ_comp_renaming_def, renaming_shift_def_termₘ. reflexivity.
+Qed.
+
+Lemma substitutionₘ_up_substitutionₘ_of_renaming {μ Γ Δ} :
+  ∀ α (σ : renaming Γ Δ),
+  substitutionₘ_up α (@substitutionₘ_of_renaming μ _ _ σ) = substitutionₘ_of_renaming (renaming_cons α MIO (renaming_comp σ (renaming_shift α Γ))).
+Proof.
+  intros α σ. rewrite substitutionₘ_up_def, renaming_cons_def_termₘ, renaming_comp_def_termₘ, substitutionₘ_comp_renaming_def. unfold substitutionₘ_shift. reflexivity.
+Qed.
+
+Lemma substitutionₘ_inst_kₘ {μ Γ Δ} :
+  ∀ (σ : substitutionₘ μ Γ Δ) n,
+  substitutionₘ_inst σ (kₘ n) = kₘ n.
+Proof.
+  intros σ n. ltac1:(simp substitutionₘ_inst'). reflexivity.
+Qed.
+
+Lemma substitutionₘ_inst_Pₘ {μ Γ Δ} :
+  ∀ (σ : substitutionₘ μ Γ Δ),
+  substitutionₘ_inst σ Pₘ = Pₘ.
+Proof.
+  intros σ. ltac1:(simp substitutionₘ_inst'). reflexivity.
+Qed.
+
+Lemma substitutionₘ_inst_Sₘ {μ Γ Δ} :
+  ∀ (σ : substitutionₘ μ Γ Δ),
+  substitutionₘ_inst σ Sₘ = Sₘ.
+Proof.
+  intros σ. ltac1:(simp substitutionₘ_inst'). reflexivity.
+Qed.
+
+Lemma substitutionₘ_inst_switchₘ {μ Γ Δ} :
+  ∀ (σ : substitutionₘ μ Γ Δ) (s' : termₘ μ Δ ι) (f : Zm μ →₀ termₘ μ Δ ι),
+  substitutionₘ_inst σ (switchₘ s' f) = switchₘ (substitutionₘ_inst σ s') (stabilizing_fun_map (substitutionₘ_inst σ) f).
+Proof.
+  intros σ s' f. ltac1:(simp substitutionₘ_inst'). reflexivity.
+Qed.
+
+Lemma substitutionₘ_inst_fixₘ {μ Γ Δ} :
+  ∀ (σ : substitutionₘ μ Γ Δ) α,
+  substitutionₘ_inst σ (fixₘ α) = fixₘ α.
+Proof.
+  intros σ α. ltac1:(simp substitutionₘ_inst'). reflexivity.
+Qed.
+
+Lemma substitutionₘ_inst_Varₘ {μ Γ Δ} :
+  ∀ (σ : substitutionₘ μ Γ Δ) α mi,
+  substitutionₘ_inst σ (Varₘ α mi) = σ α mi.
+Proof.
+  intros σ α mi. ltac1:(simp substitutionₘ_inst'). reflexivity.
+Qed.
+
+Lemma substitutionₘ_inst_appₘ {μ Γ Δ α β} :
+  ∀ (σ : substitutionₘ μ Γ Δ) (s' : termₘ μ Δ (α ⇒ β)) (t' : termₘ μ Δ α),
+  substitutionₘ_inst σ (s' $ₘ t') = (substitutionₘ_inst σ s') $ₘ (substitutionₘ_inst σ t').
+Proof.
+  intros σ s' t'. ltac1:(simp substitutionₘ_inst'). reflexivity.
+Qed.
+
+Lemma substitutionₘ_inst_absₘ {μ Γ Δ α} :
+  ∀ (σ : substitutionₘ μ Γ Δ) β (s' : termₘ μ (β :: Δ) α),
+  substitutionₘ_inst σ (λₘ: β, s') = λₘ: β, substitutionₘ_inst (substitutionₘ_up β σ) s'.
+Proof.
+  intros σ β s'. ltac1:(simp substitutionₘ_inst'). reflexivity.
+Qed.
+
+Lemma substitutionₘ_inst_substitutionₘ_cons_Varₘ_MIO {μ Γ Δ} :
+  ∀ α (s : termₘ μ Γ α) (σ : substitutionₘ μ Γ Δ),
+  substitutionₘ_inst (substitutionₘ_cons α s σ) (Varₘ α MIO) = s.
+Proof.
+  intros α s σ. rewrite substitutionₘ_inst_Varₘ. ltac1:(simp substitutionₘ_cons). reflexivity.
+Qed.
+
+Lemma substitutionₘ_comp_substitutionₘ_shift_substitutionₘ_cons {μ Γ Δ} :
+  ∀ α (s : termₘ μ Γ α) (σ : substitutionₘ μ Γ Δ),
+  substitutionₘ_comp (substitutionₘ_shift α Δ) (substitutionₘ_cons α s σ) = σ.
+Proof.
+  intros α s σ. apply functional_extensionality_dep; intros β; apply functional_extensionality; intros mi.
+  unfold substitutionₘ_comp, substitutionₘ_shift, substitutionₘ_of_renaming, renaming_shift.
+  rewrite substitutionₘ_inst_Varₘ. ltac1:(simp substitutionₘ_cons). reflexivity.
+Qed.
+
+Lemma substitutionₘ_comp_substitutionₘ_cons {μ Γ Δ Θ} :
+  ∀ α (s : termₘ μ Δ α) (τ : substitutionₘ μ Δ Θ) (σ : substitutionₘ μ Γ Δ),
+  substitutionₘ_comp (substitutionₘ_cons α s τ) σ = substitutionₘ_cons α (substitutionₘ_inst σ s) (substitutionₘ_comp τ σ).
+Proof.
+  intros α s τ σ. apply functional_extensionality_dep; intros β; apply functional_extensionality; intros mi.
+  unfold substitutionₘ_comp. ltac1:(dependent elimination mi as [@MIO Θ' | @MIS γ Θ' mi']); ltac1:(simp substitutionₘ_cons); reflexivity.
+Qed.
+
+Lemma substitutionₘ_recombination {μ Γ Δ α} :
+  ∀ (σ : substitutionₘ μ Γ (α :: Δ)),
+  substitutionₘ_cons α (substitutionₘ_inst σ (Varₘ α MIO)) (substitutionₘ_comp (substitutionₘ_shift α Δ) σ) = σ.
+Proof.
+  intros σ. apply functional_extensionality_dep; intros β; apply functional_extensionality; intros mi.
+  unfold substitutionₘ_comp, substitutionₘ_shift, substitutionₘ_of_renaming, renaming_shift. ltac1:(dependent elimination mi as [@MIO Θ' | @MIS γ Θ' mi']); ltac1:(simp substitutionₘ_cons); rewrite substitutionₘ_inst_Varₘ; reflexivity.
+Qed.
+
+Lemma substitutionₘ_cons_Varₘ_MIO_substitutionₘ_shift {μ Γ α} :
+  substitutionₘ_cons α (@Varₘ μ _ α MIO) (substitutionₘ_shift α Γ) = substitutionₘ_id (α :: Γ).
+Proof.
+  apply functional_extensionality_dep; intros β; apply functional_extensionality; intros mi.
+  unfold substitutionₘ_comp, substitutionₘ_shift, substitutionₘ_id, substitutionₘ_of_renaming, renaming_shift, renaming_id. ltac1:(dependent elimination mi as [@MIO Γ' | @MIS γ Γ' mi']); ltac1:(simp substitutionₘ_cons); reflexivity.
+Qed.
+
+Lemma substitutionₘ_comp_substitutionₘ_id_left {μ Γ Δ} :
+  ∀ (σ : substitutionₘ μ Γ Δ),
+  substitutionₘ_comp (substitutionₘ_id Δ) σ = σ.
+Proof.
+  intros σ. apply functional_extensionality_dep; intros α; apply functional_extensionality; intros mi.
+  unfold substitutionₘ_comp, substitutionₘ_id, substitutionₘ_of_renaming, renaming_id. rewrite substitutionₘ_inst_Varₘ. reflexivity.
+Qed.
+
+Lemma substitutionₘ_comp_substitutionₘ_id_right {μ Γ Δ} :
+  ∀ (σ : substitutionₘ μ Γ Δ),
+  substitutionₘ_comp σ (substitutionₘ_id Γ) = σ.
+Proof.
+  intros σ. apply functional_extensionality_dep; intros α; apply functional_extensionality; intros mi.
+  unfold substitutionₘ_comp. generalize (σ α mi) as s; intros s; clear σ mi.
+  induction s as [Γ n | Γ | Γ | Γ s' IH_s' f IH_f IH_f_default | Γ α | Γ α mi | Γ α β s' IH_s' t' IH_t' | Γ α β s' IH_s'].
+  - rewrite substitutionₘ_inst_kₘ. reflexivity.
+  - rewrite substitutionₘ_inst_Pₘ. reflexivity.
+  - rewrite substitutionₘ_inst_Sₘ. reflexivity.
+  - rewrite substitutionₘ_inst_switchₘ. rewrite IH_s'. f_equal. apply stabilizing_fun_map_id.
+    + intros n. rewrite IH_f. reflexivity.
+    + destruct (stabilizing_fun_default f) as [t' |].
+      * simpl. rewrite IH_f_default. reflexivity.
+      * reflexivity.
+  - rewrite substitutionₘ_inst_fixₘ. reflexivity.
+  - rewrite substitutionₘ_inst_Varₘ. unfold substitutionₘ_id, substitutionₘ_of_renaming, renaming_id. reflexivity.
+  - rewrite substitutionₘ_inst_appₘ. rewrite IH_s', IH_t'. reflexivity.
+  - rewrite substitutionₘ_inst_absₘ. rewrite substitutionₘ_up_def, substitutionₘ_comp_substitutionₘ_id_left, substitutionₘ_cons_Varₘ_MIO_substitutionₘ_shift. rewrite IH_s'. reflexivity.
+Qed.
+
+Lemma substitutionₘ_inst_substitutionₘ_inst_substitutionₘ_of_renaming {μ Γ Δ Θ α} :
+  ∀ (τ : renaming Δ Θ) (σ : substitutionₘ μ Γ Δ) (s : termₘ μ Θ α),
+  substitutionₘ_inst σ (substitutionₘ_inst (substitutionₘ_of_renaming τ) s) = substitutionₘ_inst (substitutionₘ_comp (substitutionₘ_of_renaming τ) σ) s.
+Proof.
+  intros τ σ s. revert Γ Δ τ σ; induction s as [Θ n | Θ | Θ | Θ s' IH_s' f IH_f IH_f_default | Θ α | Θ α mi | Θ α β s' IH_s' t' IH_t' | Θ α β s' IH_s']; intros Γ Δ τ σ.
+  - rewrite ! substitutionₘ_inst_kₘ. reflexivity.
+  - rewrite ! substitutionₘ_inst_Pₘ. reflexivity.
+  - rewrite ! substitutionₘ_inst_Sₘ. reflexivity.
+  - rewrite ! substitutionₘ_inst_switchₘ. rewrite IH_s'. f_equal. rewrite stabilizing_fun_map_stabilizing_fun_map. apply eq_stabilizing_fun_map.
+    + intros n. rewrite IH_f. reflexivity.
+    + destruct (stabilizing_fun_default f) as [t' |].
+      * simpl. rewrite IH_f_default. reflexivity.
+      * reflexivity.
+  - rewrite ! substitutionₘ_inst_fixₘ. reflexivity.
+  - rewrite ! substitutionₘ_inst_Varₘ. unfold substitutionₘ_comp. reflexivity.
+  - rewrite ! substitutionₘ_inst_appₘ. rewrite IH_s', IH_t'. reflexivity.
+  - rewrite ! substitutionₘ_inst_absₘ. rewrite (substitutionₘ_up_substitutionₘ_of_renaming β τ). rewrite IH_s'. do 2 f_equal.
+    rewrite (substitutionₘ_up_def β (substitutionₘ_comp (substitutionₘ_of_renaming τ) σ)), renaming_cons_def_termₘ, substitutionₘ_comp_substitutionₘ_cons. f_equal.
+    apply functional_extensionality_dep; intros γ; apply functional_extensionality; intros mi.
+    rewrite substitutionₘ_up_def. unfold substitutionₘ_comp at 1 3 4, renaming_comp, substitutionₘ_of_renaming. rewrite ! substitutionₘ_inst_Varₘ.
+    specialize (substitutionₘ_comp_substitutionₘ_shift_substitutionₘ_cons β (Varₘ β MIO) (substitutionₘ_comp σ (substitutionₘ_shift β Γ))) as H. specialize (equal_f (equal_f_dep H γ) (τ γ mi)) as H'.
+    unfold substitutionₘ_comp at 1 3, substitutionₘ_shift, substitutionₘ_of_renaming at 2 in H'. rewrite substitutionₘ_inst_Varₘ in H'.
+    unfold substitutionₘ_shift. rewrite H'. reflexivity.
+Qed.
+
+Lemma substitutionₘ_inst_substitutionₘ_of_renaming_substitutionₘ_inst {μ Γ Δ Θ α} :
+  ∀ (τ : substitutionₘ μ Δ Θ) (σ : renaming Γ Δ) (s : termₘ μ Θ α),
+  substitutionₘ_inst (substitutionₘ_of_renaming σ) (substitutionₘ_inst τ s) = substitutionₘ_inst (substitutionₘ_comp τ (substitutionₘ_of_renaming σ)) s.
+Proof.
+  intros τ σ s. revert Γ Δ τ σ; induction s as [Θ n | Θ | Θ | Θ s' IH_s' f IH_f IH_f_default | Θ α | Θ α mi | Θ α β s' IH_s' t' IH_t' | Θ α β s' IH_s']; intros Γ Δ τ σ.
+  - rewrite ! substitutionₘ_inst_kₘ. reflexivity.
+  - rewrite ! substitutionₘ_inst_Pₘ. reflexivity.
+  - rewrite ! substitutionₘ_inst_Sₘ. reflexivity.
+  - rewrite ! substitutionₘ_inst_switchₘ. rewrite IH_s'. f_equal. rewrite stabilizing_fun_map_stabilizing_fun_map. apply eq_stabilizing_fun_map.
+    + intros n. rewrite IH_f. reflexivity.
+    + destruct (stabilizing_fun_default f) as [t' |].
+      * simpl. rewrite IH_f_default. reflexivity.
+      * reflexivity.
+  - rewrite ! substitutionₘ_inst_fixₘ. reflexivity.
+  - rewrite ! substitutionₘ_inst_Varₘ. unfold substitutionₘ_comp. reflexivity.
+  - rewrite ! substitutionₘ_inst_appₘ. rewrite IH_s', IH_t'. reflexivity.
+  - rewrite ! substitutionₘ_inst_absₘ. rewrite (substitutionₘ_up_substitutionₘ_of_renaming β σ). rewrite IH_s'. do 2 f_equal.
+    rewrite ! substitutionₘ_up_def, renaming_cons_def_termₘ, substitutionₘ_comp_substitutionₘ_cons. f_equal.
+    apply functional_extensionality_dep; intros γ; apply functional_extensionality; intros mi.
+    unfold substitutionₘ_comp, substitutionₘ_shift. rewrite ! substitutionₘ_inst_substitutionₘ_inst_substitutionₘ_of_renaming.
+    specialize (@substitutionₘ_comp_substitutionₘ_shift_substitutionₘ_cons μ _ _ β (Varₘ β MIO) (substitutionₘ_of_renaming (renaming_comp σ (renaming_shift β Γ)))) as H. unfold substitutionₘ_shift in H. rewrite H.
+    rewrite renaming_comp_def_termₘ, substitutionₘ_comp_renaming_def. reflexivity.
+Qed.
+
+Lemma substitutionₘ_inst_substitutionₘ_inst {μ Γ Δ Θ α} :
+  ∀ (τ : substitutionₘ μ Δ Θ) (σ : substitutionₘ μ Γ Δ) (s : termₘ μ Θ α),
+  substitutionₘ_inst σ (substitutionₘ_inst τ s) = substitutionₘ_inst (substitutionₘ_comp τ σ) s.
+Proof.
+  intros τ σ s. revert Γ Δ τ σ; induction s as [Θ n | Θ | Θ | Θ s' IH_s' f IH_f IH_f_default | Θ α | Θ α mi | Θ α β s' IH_s' t' IH_t' | Θ α β s' IH_s']; intros Γ Δ τ σ.
+  - rewrite ! substitutionₘ_inst_kₘ. reflexivity.
+  - rewrite ! substitutionₘ_inst_Pₘ. reflexivity.
+  - rewrite ! substitutionₘ_inst_Sₘ. reflexivity.
+  - rewrite ! substitutionₘ_inst_switchₘ. rewrite IH_s'. f_equal. rewrite stabilizing_fun_map_stabilizing_fun_map. apply eq_stabilizing_fun_map.
+    + intros n. rewrite IH_f. reflexivity.
+    + destruct (stabilizing_fun_default f) as [t' |].
+      * simpl. rewrite IH_f_default. reflexivity.
+      * reflexivity.
+  - rewrite ! substitutionₘ_inst_fixₘ. reflexivity.
+  - rewrite ! substitutionₘ_inst_Varₘ. unfold substitutionₘ_comp. reflexivity.
+  - rewrite ! substitutionₘ_inst_appₘ. rewrite IH_s', IH_t'. reflexivity.
+  - rewrite ! substitutionₘ_inst_absₘ. rewrite IH_s'. do 2 f_equal.
+    rewrite (substitutionₘ_up_def β τ), (substitutionₘ_up_def β (substitutionₘ_comp τ σ)), substitutionₘ_comp_substitutionₘ_cons. f_equal.
+    apply functional_extensionality_dep; intros γ; apply functional_extensionality; intros mi.
+    unfold substitutionₘ_comp, substitutionₘ_shift.
+    rewrite substitutionₘ_inst_substitutionₘ_inst_substitutionₘ_of_renaming, substitutionₘ_inst_substitutionₘ_of_renaming_substitutionₘ_inst, substitutionₘ_up_def.
+    specialize (@substitutionₘ_comp_substitutionₘ_shift_substitutionₘ_cons μ _ _ β (Varₘ β MIO) (substitutionₘ_comp σ (substitutionₘ_shift β Γ))) as H. unfold substitutionₘ_shift in H |- *. rewrite H. reflexivity.
+Qed.
+
+Lemma associativity_rev_substitutionₘ_comp {μ Γ Δ Θ Λ} :
+  ∀ (υ : substitutionₘ μ Θ Λ) (τ : substitutionₘ μ Δ Θ) (σ : substitutionₘ μ Γ Δ),
+  substitutionₘ_comp (substitutionₘ_comp υ τ) σ = substitutionₘ_comp υ (substitutionₘ_comp τ σ).
+Proof.
+  intros υ τ σ. apply functional_extensionality_dep; intros α; apply functional_extensionality; intros mi.
+  unfold substitutionₘ_comp at 1 2 3. rewrite substitutionₘ_inst_substitutionₘ_inst. reflexivity.
+Qed.
+
+Hint Rewrite @renaming_id_def_termₘ : substitutionₘ.
+Hint Rewrite @renaming_cons_def_termₘ : substitutionₘ.
+Hint Rewrite @renaming_shift_def_termₘ : substitutionₘ.
+Hint Rewrite @renaming_comp_def_termₘ : substitutionₘ.
+Hint Rewrite @renaming_up_def_termₘ : substitutionₘ.
+Hint Rewrite @renaming_inst_termₘ_def : substitutionₘ.
+Hint Rewrite @substitutionₘ_comp_renaming_def : substitutionₘ.
+Hint Rewrite @substitutionₘ_up_def : substitutionₘ.
+Hint Rewrite @substitutionₘ_up_substitutionₘ_of_renaming : substitutionₘ.
+Hint Rewrite @substitutionₘ_inst_kₘ : substitutionₘ.
+Hint Rewrite @substitutionₘ_inst_Pₘ : substitutionₘ.
+Hint Rewrite @substitutionₘ_inst_Sₘ : substitutionₘ.
+Hint Rewrite @substitutionₘ_inst_switchₘ : substitutionₘ.
+Hint Rewrite @substitutionₘ_inst_fixₘ : substitutionₘ.
+Hint Rewrite @substitutionₘ_inst_appₘ : substitutionₘ.
+Hint Rewrite @substitutionₘ_inst_absₘ : substitutionₘ.
+Hint Rewrite @substitutionₘ_inst_substitutionₘ_cons_Varₘ_MIO : substitutionₘ.
+Hint Rewrite @substitutionₘ_comp_substitutionₘ_shift_substitutionₘ_cons : substitutionₘ.
+Hint Rewrite @substitutionₘ_comp_substitutionₘ_cons : substitutionₘ.
+Hint Rewrite @substitutionₘ_recombination : substitutionₘ.
+Hint Rewrite @substitutionₘ_comp_substitutionₘ_id_left : substitutionₘ.
+Hint Rewrite @substitutionₘ_cons_Varₘ_MIO_substitutionₘ_shift : substitutionₘ.
+Hint Rewrite @substitutionₘ_comp_substitutionₘ_id_left : substitutionₘ.
+Hint Rewrite @substitutionₘ_comp_substitutionₘ_id_right : substitutionₘ.
+Hint Rewrite @associativity_rev_substitutionₘ_comp : substitutionₘ.
+
 Reserved Notation "s_1  ⟶ₘ  s_2" (at level 70).
 
-Inductive termₘ_step {μ} : ∀ {Γ α}, termₘ μ Γ α → termₘ μ Γ α → Prop :=
-  | termₘ_step_switchₘ_cong :
-    ∀ {Γ} (s'_1 s'_2 : termₘ μ Γ ι) (f_1 f_2 : Zm μ →₀ termₘ μ Γ ι),
+Inductive termₘ_step {μ} : ∀ {Γ α}, termₘ μ Γ α → termₘ μ Γ α → Type :=
+  | termₘ_step_Pₘ :
+    ∀ {Γ} n,
+    (@Pₘ _ Γ) $ₘ (kₘ n) ⟶ₘ kₘ (Zm_pred n)
+  | termₘ_step_Sₘ :
+    ∀ {Γ} n,
+    (@Sₘ _ Γ) $ₘ (kₘ n) ⟶ₘ kₘ (Zm_succ n)
+  | termₘ_step_switchₘ_s' :
+    ∀ {Γ} (s'_1 s'_2 : termₘ μ Γ ι) (f : Zm μ →₀ termₘ μ Γ ι),
     s'_1 ⟶ₘ s'_2 →
-    (∀ n, f_1 n ⟶ₘ f_2 n) →
-    switchₘ s'_1 f_1 ⟶ₘ switchₘ s'_2 f_2
-  | termₘ_step_Appₘ :
-    ∀ {Γ α β} (s'_1 s'_2 : termₘ μ Γ (α ⇒ β)) (t'_1 t'_2 : termₘ μ Γ α),
-    s'_1 ⟶ₘ s'_2 →
+    switchₘ s'_1 f ⟶ₘ switchₘ s'_2 f
+  | termₘ_step_switchₘ_f :
+    ∀ {Γ} (s' : termₘ μ Γ ι) (f : Zm μ →₀ termₘ μ Γ ι),
+    ¬ stabilizing_fun_canonical f →
+    switchₘ s' f ⟶ₘ switchₘ s' (stabilizing_fun_canonize f)
+  | termₘ_step_switchₘ_f_n :
+    ∀ {Γ} (s' : termₘ μ Γ ι) (f : Zm μ →₀ termₘ μ Γ ι) n (t' : termₘ μ Γ ι),
+    stabilizing_fun_canonical f →
+    f n ⟶ₘ t' →
+    switchₘ s' f ⟶ₘ switchₘ s' (n ↦₀ t', f)
+  | termₘ_step_switchₘ_f_default :
+    ∀ {Γ} (s' : termₘ μ Γ ι) (f : Zm μ →₀ termₘ μ Γ ι) (t'_1 t'_2 : termₘ μ Γ ι),
+    stabilizing_fun_canonical f →
+    stabilizing_fun_default f = Some t'_1 →
     t'_1 ⟶ₘ t'_2 →
-    Appₘ s'_1 t'_1 ⟶ₘ Appₘ s'_2 t'_2
-  | termₘ_step_Absₘ :
-    ∀ {Γ α β} (s'_1 s'_2 : termₘ μ (β :: Γ) α),
+    switchₘ s' f ⟶ₘ switchₘ s' (_ ↦₀ t'_2, f)
+  | termₘ_step_switchₘ :
+    ∀ {Γ} n (f : Zm μ →₀ termₘ μ Γ ι),
+    switchₘ (kₘ n) f ⟶ₘ f n
+  | termₘ_step_fixₘ :
+    ∀ {Γ} α (s : termₘ μ Γ (α ⇒ α)),
+    fixₘ α $ₘ s ⟶ₘ s $ₘ (fixₘ α $ₘ s)
+  | termₘ_step_Appₘ_s' :
+    ∀ {Γ α β} (s'_1 s'_2 : termₘ μ Γ (α ⇒ β)) (t' : termₘ μ Γ α),
     s'_1 ⟶ₘ s'_2 →
-    Absₘ β s'_1 ⟶ₘ Absₘ β s'_2
+    s'_1 $ₘ t' ⟶ₘ s'_2 $ₘ t'
+  | termₘ_step_Appₘ_t' :
+    ∀ {Γ α β} (s' : termₘ μ Γ (α ⇒ β)) (t'_1 t'_2 : termₘ μ Γ α),
+    t'_1 ⟶ₘ t'_2 →
+    s' $ₘ t'_1 ⟶ₘ s' $ₘ t'_2
+  | termₘ_step_Absₘ_s' :
+    ∀ {Γ α} β (s'_1 s'_2 : termₘ μ (β :: Γ) α),
+    s'_1 ⟶ₘ s'_2 →
+    λₘ: β, s'_1 ⟶ₘ λₘ: β, s'_2
+  | termₘ_step_Absₘ :
+    ∀ {Γ α} β (s' : termₘ μ (β :: Γ) α) (t : termₘ μ Γ β),
+    (λₘ: β, s') $ₘ t ⟶ₘ substitutionₘ_inst (substitutionₘ_cons β t (substitutionₘ_id Γ)) s'
   where "s_1 ⟶ₘ s_2" := (termₘ_step s_1 s_2).
+
+Definition termₘ_red {μ Γ α} := t_closure_t (@termₘ_step μ Γ α).
+
+Notation "s_1  ⟶⁺ₘ  s_2" := (termₘ_red s_1 s_2) (at level 70).
+
+Inductive termₘ_normal {μ Γ} : ∀ {α}, termₘ μ Γ α → Type :=
+  | termₘ_normal_of_termₘ_neutral :
+    ∀ {α} (s : termₘ μ Γ α),
+    termₘ_neutral s →
+    termₘ_normal s
+  | termₘ_normal_kₘ :
+    ∀ n,
+    termₘ_normal (kₘ n)
+  | termₘ_normal_Pₘ :
+    termₘ_normal Pₘ
+  | termₘ_normal_Sₘ :
+    termₘ_normal Sₘ
+  | termₘ_normal_fixₘ :
+    ∀ α,
+    termₘ_normal (fixₘ α)
+  | termₘ_normal_Absₘ :
+    ∀ {α} β (s' : termₘ μ (β :: Γ) α),
+    termₘ_normal s' →
+    termₘ_normal (λₘ: β, s')
+with termₘ_neutral {μ Γ} : ∀ {α}, termₘ μ Γ α → Type :=
+  | termₘ_neutral_Pₘ :
+    ∀ (s : termₘ μ Γ ι),
+    termₘ_neutral s →
+    termₘ_neutral (Pₘ $ₘ s)
+  | termₘ_neutral_Sₘ :
+    ∀ (s : termₘ μ Γ ι),
+    termₘ_neutral s →
+    termₘ_neutral (Sₘ $ₘ s)
+  | termₘ_neutral_switchₘ :
+    ∀ (s : termₘ μ Γ ι) (f : Zm μ →₀ termₘ μ Γ ι),
+    termₘ_neutral s →
+    (∀ n, termₘ_normal (f n)) →
+    termₘ_neutral (switchₘ s f)
+  | termₘ_neutral_Varₘ :
+    ∀ {α} (mi : mem_index α Γ),
+    termₘ_neutral (Varₘ α mi)
+  | termₘ_neutral_Appₘ :
+    ∀ {α β} (s' : termₘ μ Γ (α ⇒ β)) (t' : termₘ μ Γ α),
+    termₘ_neutral s' →
+    termₘ_normal t' →
+    termₘ_neutral (s' $ₘ t').
+
+Scheme termₘ_normal_mutind := Induction for termₘ_normal Sort Prop
+with termₘ_neutral_mutind := Induction for termₘ_neutral Sort Prop.
+
+Scheme termₘ_normal_mutrect := Induction for termₘ_normal Sort Type
+with termₘ_neutral_mutrect := Induction for termₘ_neutral Sort Type.
+
+Definition termₘ_normal_mutrec μ (P_normal : ∀ Γ α (s : termₘ μ Γ α), termₘ_normal s → Set) (P_neutral : ∀ Γ α (s : termₘ μ Γ α), termₘ_neutral s → Set) := termₘ_normal_mutrect μ P_normal P_neutral.
+Definition termₘ_neutral_mutrec μ (P_normal : ∀ Γ α (s : termₘ μ Γ α), termₘ_normal s → Set) (P_neutral : ∀ Γ α (s : termₘ μ Γ α), termₘ_neutral s → Set) := termₘ_neutral_mutrect μ P_normal P_neutral.
+
+Definition termₘ_progress {μ Γ α} (s : termₘ μ Γ α) : {t & s ⟶ₘ t} + termₘ_normal s.
+Proof.
+  induction s as [Γ n | Γ | Γ | Γ s'_1 IH_s' f_1 IH_f IH_f_default | Γ α | Γ α mi | Γ α β s'_1 IH_s' t'_1 IH_t' | Γ α β s'_1 IH_s'].
+  - right. apply termₘ_normal_kₘ.
+  - right. apply termₘ_normal_Pₘ.
+  - right. apply termₘ_normal_Sₘ.
+  - destruct (dec_stabilizing_fun_canonical f_1) as [canonical_f_1 | canonical_f_1].
+    + assert (H_f : {n & {t'_2 & f_1 n ⟶ₘ t'_2}} + (∀ n, mem_index n (stabilizing_fun_keys f_1) → termₘ_normal (f_1 n))). {
+        clear s'_1 IH_f_default IH_s' canonical_f_1. generalize (stabilizing_fun_keys f_1); intros f_keys. induction f_keys as [| n f_keys' IH_f_keys].
+        - right. intros n H. inversion H.
+        - destruct (IH_f n) as [H_f_n | H_f_n] > [| destruct IH_f_keys as [(m & IH_f_keys) | IH_f_keys]].
+          + left. exists n. auto.
+          + left. exists m. auto.
+          + right. intros m mi. inversion mi; auto.
+      }
+      remember (stabilizing_fun_default f_1) as f_1_default eqn:H_f_1_default; symmetry in H_f_1_default.
+      destruct IH_s' as [(s'_2 & H_s') | H_s'].
+      * left. exists (switchₘ s'_2 f_1). apply termₘ_step_switchₘ_s'; auto.
+      * ltac1:(dependent elimination H_s' as [termₘ_normal_of_termₘ_neutral s'_1 H_s' | termₘ_normal_kₘ n]).
+        -- destruct H_f as [(n & t'_2 & H_f_n) | H_f_n] > [| destruct f_1_default as [t'_1 |] > [destruct IH_f_default as [(t'_2 & H_f_default) | H_f_default] |]].
+           ++ left. exists (switchₘ s'_1 (n ↦₀ t'_2, f_1)). apply termₘ_step_switchₘ_f_n; auto.
+           ++ left. exists (switchₘ s'_1 (_ ↦₀ t'_2, f_1)). apply termₘ_step_switchₘ_f_default with t'_1; auto.
+           ++ right. apply termₘ_normal_of_termₘ_neutral, termₘ_neutral_switchₘ > [auto |]. intros n.
+              unfold stabilizing_fun_canonical in canonical_f_1. rewrite H_f_1_default in canonical_f_1. destruct canonical_f_1 as (_ & _ & canonical_f_1).
+              destruct (dec_eq_list_In n (stabilizing_fun_keys f_1)) as [mi | H_n].
+              ** apply H_f_n, mi.
+              ** specialize (canonical_f_1 n). destruct (f_1 n == t'_1) as [-> | H_f_1_n] > [| ltac1:(intuition auto)]. auto.
+           ++ right. apply termₘ_normal_of_termₘ_neutral, termₘ_neutral_switchₘ > [auto |]. intros n.
+              unfold stabilizing_fun_canonical in canonical_f_1. rewrite H_f_1_default in canonical_f_1. destruct canonical_f_1 as (_ & _ & canonical_f_1).
+              destruct (dec_eq_list_In n (stabilizing_fun_keys f_1)) as [mi | H_n].
+              ** apply H_f_n, mi.
+              ** specialize (canonical_f_1 n). exfalso. auto.
+        -- left. exists (f_1 n). apply termₘ_step_switchₘ.
+    + left. exists (switchₘ s'_1 (stabilizing_fun_canonize f_1)). apply termₘ_step_switchₘ_f; auto.
+  - right. apply termₘ_normal_fixₘ.
+  - right. apply termₘ_normal_of_termₘ_neutral, termₘ_neutral_Varₘ.
+  - ltac1:(dependent elimination s'_1 as [@Pₘ Γ | @Sₘ Γ | @fixₘ Γ s'_α | @Varₘ Γ s'_α s'_mi | @Appₘ Γ s'_α s'_β s'_s' s'_t' | @Absₘ Γ s'_α s'_β s'_s']).
+    + destruct IH_s' as [(s'_2 & H_s') | H_s'] > [| destruct IH_t' as [(t'_2 & H_t') | H_t']].
+      * left. exists (s'_2 $ₘ t'_1). apply termₘ_step_Appₘ_s'; auto.
+      * left. exists (Pₘ $ₘ t'_2). apply termₘ_step_Appₘ_t'; auto.
+      * ltac1:(dependent elimination H_t' as [termₘ_normal_of_termₘ_neutral t'_1 H_t' | termₘ_normal_kₘ n]).
+        -- right. apply termₘ_normal_of_termₘ_neutral, termₘ_neutral_Pₘ; auto.
+        -- left. exists (kₘ (Zm_pred n)). apply termₘ_step_Pₘ.
+    + destruct IH_s' as [(s'_2 & H_s') | H_s'] > [| destruct IH_t' as [(t'_2 & H_t') | H_t']].
+      * left. exists (s'_2 $ₘ t'_1). apply termₘ_step_Appₘ_s'; auto.
+      * left. exists (Sₘ $ₘ t'_2). apply termₘ_step_Appₘ_t'; auto.
+      * ltac1:(dependent elimination H_t' as [termₘ_normal_of_termₘ_neutral t'_1 H_t' | termₘ_normal_kₘ n]).
+        -- right. apply termₘ_normal_of_termₘ_neutral, termₘ_neutral_Sₘ; auto.
+        -- left. exists (kₘ (Zm_succ n)). apply termₘ_step_Sₘ.
+    + left. exists (t'_1 $ₘ (fixₘ s'_α $ₘ t'_1)). apply termₘ_step_fixₘ.
+    + destruct IH_s' as [(s'_2 & H_s') | H_s'] > [| destruct IH_t' as [(t'_2 & H_t') | H_t']].
+      * left. exists (s'_2 $ₘ t'_1). apply termₘ_step_Appₘ_s'; auto.
+      * left. exists (Varₘ (α ⇒ β) s'_mi $ₘ t'_2). apply termₘ_step_Appₘ_t'; auto.
+      * ltac1:(dependent elimination H_s' as [termₘ_normal_of_termₘ_neutral _ H_s']).
+        right. apply termₘ_normal_of_termₘ_neutral, termₘ_neutral_Appₘ; auto.
+    + destruct IH_s' as [(s'_2 & H_s') | H_s'] > [| destruct IH_t' as [(t'_2 & H_t') | H_t']].
+      * left. exists (s'_2 $ₘ t'_1). apply termₘ_step_Appₘ_s'; auto.
+      * left. exists (s'_s' $ₘ s'_t' $ₘ t'_2). apply termₘ_step_Appₘ_t'; auto.
+      * ltac1:(dependent elimination H_s' as [termₘ_normal_of_termₘ_neutral _ H_s']).
+        right. apply termₘ_normal_of_termₘ_neutral, termₘ_neutral_Appₘ; auto.
+    + left. exists (substitutionₘ_inst (substitutionₘ_cons s'_β t'_1 (substitutionₘ_id Γ)) s'_s'). apply termₘ_step_Absₘ.
+  - destruct IH_s' as [(s'_2 & H_s') | H_s'].
+    + left. exists (λₘ: β, s'_2). apply termₘ_step_Absₘ_s'; auto.
+    + right. apply termₘ_normal_Absₘ; auto.
+Defined.
+
+Lemma termₘ_normal_termₘ_step {μ Γ α} :
+  ∀ (s t : termₘ μ Γ α),
+  termₘ_normal s →
+  s ⟶ₘ t →
+  False.
+Proof.
+Admitted.
+
+Fixpoint termₘ_reduce {μ Γ α} (n : nat) (s : termₘ μ Γ α) : option {t : termₘ μ Γ α & (s ⟶⁺ₘ t)}.
+Proof.
+  destruct n as [| n'].
+  - apply None.
+  - destruct (termₘ_progress s) as [(t & H_s) | H_s].
+    + apply t_closure_t_step in H_s. destruct (termₘ_reduce _ _ _ n' t) as [(u & H_t) |].
+      * apply Some. exists u. apply trans_t_closure_t with t; auto.
+      * apply Some. exists t. auto.
+    + apply None.
+Defined.
+
+Definition termₘ_reduce_list {μ Γ α} (n : nat) (s : termₘ μ Γ α) : list (termₘ μ Γ α) :=
+  s ::
+  match termₘ_reduce n s with
+  | None => []
+  | Some (existT _ _ H) => list_of_t_closure_t H
+  end.
+
+Definition example_plusₘ {μ Γ} : termₘ μ Γ (ι ⇒ ι ⇒ ι) :=
+  fixₘ (ι ⇒ ι ⇒ ι) $ₘ (λₘ: ι ⇒ ι ⇒ ι, λₘ: ι, λₘ: ι,
+    switchₘ (Varₘ ι (MIS MIO)) (
+      Zm_of_Z 0 ↦₀ Varₘ ι MIO,
+      _ ↦₀ Sₘ $ₘ (Varₘ (ι ⇒ ι ⇒ ι) (MIS (MIS MIO)) $ₘ (Pₘ $ₘ Varₘ ι (MIS MIO)) $ₘ (Varₘ ι (MIS MIO)))
+    )
+  ).
+
+Definition example_fibonacciₘ {μ Γ} : termₘ μ Γ (ι ⇒ ι) :=
+  fixₘ (ι ⇒ ι) $ₘ (λₘ: ι ⇒ ι, λₘ: ι,
+    switchₘ (Varₘ ι MIO) (
+      Zm_of_Z 0 ↦₀ kₘ (Zm_of_Z 1),
+      Zm_of_Z 1 ↦₀ kₘ (Zm_of_Z 1),
+      _ ↦₀ example_plusₘ $ₘ (Varₘ (ι ⇒ ι) (MIS MIO) $ₘ (Pₘ $ₘ (Pₘ $ₘ (Varₘ ι MIO)))) $ₘ (Pₘ $ₘ (Varₘ ι MIO))
+    )
+  ).
+
+Eval lazy in (List.map rebuild_termₘ (termₘ_reduce_list 3 (@example_fibonacciₘ 0 [] $ₘ (kₘ (Zm_of_Z 7))))).
+
+(*
+Set Printing Width 120.
+Set Printing Depth 10000.
+Eval lazy in (List.map rebuild_termₘ (termₘ_reduce_list 1000 (@example_fibonacciₘ 0 [] $ₘ (kₘ (Zm_of_Z 3))))).
+*)
